Backing up more partial work

src/api/dotnet/Keyring.cs
@@ -1,5 +1,0 @@
-namespace AWSEncryptionSDK {
-    public interface Keyring {
-        
-    }
-}
