src/extern/dotnet/StandardLibrary.cs
@@ -1,0 +1,13 @@
+namespace STL {
+
+  public partial class __default {
+    public static Option<T> As<T>(object x) where T : class {
+      var casted = x as T;
+      if (casted != null) {
+        return Option<T>.create_Some(casted);
+      } else {
+        return Option<T>.create_None();
+      }
+    }
+  }
+}
