src/SDK/Materials.dfy
@@ -131,6 +131,13 @@ module {:extern "Materials"} Materials {
 
   type ValidEncryptionMaterials = i: EncryptionMaterials | i.Valid() witness EncryptionMaterials.ValidWitness()
 
+  class {:extern} ExternalEncryptionMaterials {
+    const wrapped: ValidEncryptionMaterials
+    constructor(wrapped: ValidEncryptionMaterials) {
+      this.wrapped := wrapped;
+    }
+  }
+
   datatype DecryptionMaterials = DecryptionMaterials(algorithmSuiteID: AlgorithmSuite.ID,
                                                      encryptionContext: EncryptionContext,
                                                      plaintextDataKey: Option<seq<uint8>>,
@@ -178,6 +185,13 @@ module {:extern "Materials"} Materials {
   }
 
   type ValidDecryptionMaterials = i: DecryptionMaterials | i.Valid() witness DecryptionMaterials.ValidWitness()
+
+  class {:extern} ExternalDecryptionMaterials {
+    const wrapped: ValidDecryptionMaterials
+    constructor(wrapped: ValidDecryptionMaterials) {
+      this.wrapped := wrapped;
+    }
+  }
 
   datatype EncryptionMaterialsRequest = EncryptionMaterialsRequest(encryptionContext: EncryptionContext,
                                                                    algorithmSuiteID: Option<AlgorithmSuite.ID>,
